library/init/meta/decl_cmds.lean
@@ -37,7 +37,7 @@ e^.replace (λ e d,
         lemma g_lemma : forall a, g a > 0 := ... -/
 meta def copy_decl_updating_type (replacements : name_map name) (src_decl_name : name) (new_decl_name : name) : command :=
 do env  ← get_env,
-   decl ← returnex $ env^.get src_decl_name,
+   decl ← env^.get src_decl_name,
    decl ← return $ decl^.update_name $ new_decl_name,
    decl ← return $ decl^.update_type $ apply_replacement replacements decl^.type,
    decl ← return $ decl^.update_value $ expr.const src_decl_name (decl^.univ_params^.for level.param),
@@ -45,7 +45,7 @@ do env  ← get_env,
 
 meta def copy_decl_using (replacements : name_map name) (src_decl_name : name) (new_decl_name : name) : command :=
 do env  ← get_env,
-   decl ← returnex $ env^.get src_decl_name,
+   decl ← env^.get src_decl_name,
    decl ← return $ decl^.update_name $ new_decl_name,
    decl ← return $ decl^.update_type $ apply_replacement replacements decl^.type,
    decl ← return $ decl^.map_value $ apply_replacement replacements,
