tests/lean/run/assoc_flat.lean
@@ -16,15 +16,15 @@ meta definition flat_with : expr → expr → expr → expr → tactic (expr × 
     (new_app, H₂)  ← flat_with op assoc a1 rhs₁,
     -- We need to generate a proof that (a1 + a2) + rhs = a1 + (a2 + rhs)
     -- H₃ is a proof for (a1 + a2) + rhs = a1 + (a2 + rhs)
-    H₃ : expr      ← return (app (app (app assoc a1) a2) rhs),
+    H₃             ← return $ assoc a1 a2 rhs,
     -- H₃ is a proof for a1 + (a2 + rhs) = a1 + rhs1
-    H₄ : expr      ← mk_app `congr_arg [app op a1, H₁],
-    H₅             ← mk_app `eq.trans [H₃, H₄],
-    H              ← mk_app `eq.trans [H₅, H₂],
+    H₄             ← to_expr `(congr_arg %%(app op a1) %%H₁),
+    H₅             ← to_expr `(eq.trans %%H₃ %%H₄),
+    H              ← to_expr `(eq.trans %%H₅ %%H₂),
     return (new_app, H)
   | none          := do
-    new_app ← return $ app (app op e) rhs,
-    H       ← mk_app `eq.refl [new_app],
+    new_app ← return $ op e rhs,
+    H       ← to_expr `(eq.refl %%new_app),
     return (new_app, H)
   end
 
@@ -38,11 +38,11 @@ meta definition flat : expr → expr → expr → tactic (expr × expr)
     (new_app, H₂)  ← flat_with op assoc a1 new_a2,
     -- We need a proof that (a1 + a2) = new_app
     -- H₃ is a proof for a1 + a2 = a1 + new_a2
-    H₃ : expr      ← mk_app `congr_arg [app op a1, H₁],
-    H              ← mk_app `eq.trans [H₃, H₂],
+    H₃ : expr      ← to_expr `(congr_arg %%(app op a1) %%H₁),
+    H              ← to_expr `(eq.trans %%H₃ %%H₂),
     return (new_app, H)
   | none          :=
-    do pr ← mk_app `eq.refl [e],
+    do pr ← to_expr `(eq.refl %%e),
        return (e, pr)
   end
 
@@ -52,13 +52,12 @@ set_option pp.all true
 
 example (a b c d e f g : nat) : ((a + b) + c) + ((d + e) + (f + g))  = a + (b + (c + (d + (e + (f + g))))) :=
 by do
-  assoc : expr ← mk_const $ `nat.add_assoc,
-  op : expr    ← mk_const $ `nat.add,
+  assoc : expr ← mk_const `nat.add_assoc,
+  op : expr    ← mk_const `nat.add,
   tgt          ← target,
-  match (is_eq tgt) with
+  match is_eq tgt with
   | (some (lhs, rhs)) := do
     r ← flat op assoc lhs,
-    trace (prod.snd r),
-    exact (prod.snd r)
+    exact r.2
   | none            := failed
   end
